src/main-mmap.h
@@ -8,7 +8,7 @@ static uint8_t *mmap_u8(size_t len);
 
 static uint64_t *mmap_u64(size_t len);
 
-static ArrayList_cell__int32_t *mmap_cell_status(size_t len);
+// static ArrayListGen_cell__int32_t *mmap_cell_status(size_t len);
 
 static uint32_t *mmap_ptr_u32(void);
 
