src/MainMMap.fst
@@ -12,7 +12,8 @@ module AL = ArrayList
 module R = Steel.Reference
 module A = Steel.Array
 
-assume val mmap_u8 (len: US.t)
+assume
+val mmap_u8 (len: US.t)
   : Steel (array U8.t)
     emp
     (fun a -> A.varray a)
@@ -22,7 +23,9 @@ assume val mmap_u8 (len: US.t)
       A.is_full_array a /\
       A.asel a h1 == Seq.create (US.v len) U8.zero
     )
-assume val mmap_u64 (len: US.t)
+
+assume
+val mmap_u64 (len: US.t)
   : Steel (array U64.t)
     emp
     (fun a -> A.varray a)
@@ -33,22 +36,24 @@ assume val mmap_u64 (len: US.t)
       A.asel a h1 == Seq.create (US.v len) U64.zero
     )
 
-assume val mmap_cell_status (len: US.t)
-  : Steel (array AL.cell)
-     emp
-    (fun a -> A.varray a)
-    (fun _ -> True)
-    (fun _ a h1 ->
-      A.length a == US.v len /\
-      A.is_full_array a
-    )
+// val mmap_cell_status (len: US.t)
+//   : Steel (array ArrayListType.cell)
+//      emp
+//     (fun a -> A.varray a)
+//     (fun _ -> True)
+//     (fun _ a h1 ->
+//       A.length a == US.v len /\
+//       A.is_full_array a
+//     )
 
-assume val mmap_ptr_u32 (_:unit)
+assume
+val mmap_ptr_u32 (_:unit)
   : SteelT (R.ref U32.t)
     emp
     (fun r -> R.vptr r)
 
-assume val mmap_ptr_us (_:unit)
+assume
+val mmap_ptr_us (_:unit)
   : SteelT (R.ref US.t)
     emp
     (fun r -> R.vptr r)
